test/coq/incr_proof.v
@@ -60,7 +60,7 @@ Lemma Incr__spec:
   ⊢ WP eval_mexpr η Incr {{ module_spec Λ }}.
 Proof.
   iIntros.
-  wp.
+  wp. wp_bind. wp_bind.
 
   (* Prove that [new_counter] matches its specification (defined above). *)
   o_specify "new_counter" new_counter_spec "#Hnew_counter".
@@ -104,7 +104,7 @@ Proof.
 
   wp_use ("Hget" with "Hl").
   iNext. iIntros (?)"[->Hl]".
-  wp_continue.
+  wp_continue. wp_bind.
 
   wp_use ("Hupd" with "Hl").
   iNext. iIntros "Hl".
@@ -112,7 +112,7 @@ Proof.
 
   wp_use ("Hget" with "Hl").
   iNext. iIntros (?)"[->Hl]".
-  wp. wp_continue.
+  wp. wp_continue. wp_bind.
 
 
   iClear "Hget Hupd Hl". clear l.
@@ -126,7 +126,7 @@ Proof.
 
   wp_use ("Hget" with "Hl").
   iNext. iIntros (?)"[->Hl]".
-  wp_continue.
+  wp_continue. wp_bind.
 
   wp_use ("Hupd" with "Hl").
   iNext. iIntros "Hl".
@@ -135,7 +135,7 @@ Proof.
   wp_use ("Hget" with "Hl").
   iNext. iIntros (?)"[->Hl]".
 
-  wp. wp_continue.
+  wp. wp_continue. wp_bind.
 
   wp_continue.
 
